include/MacroFrontendAction.h
@@ -12,8 +12,9 @@
 
 class MacroFrontendAction : public clang::SyntaxOnlyAction {
 public:
-    explicit MacroFrontendAction(std::unordered_map<clang::FileID, std::map<unsigned, MacroEventInfo>, FileIDHash> &macroEvents)
-        : macroInfoMap(macroEvents) {}
+    explicit MacroFrontendAction(std::unordered_map<clang::FileID, std::map<unsigned, MacroEventInfo>, FileIDHash> &macroEvents,
+        std::unordered_map<unsigned, std::vector<TokenInfo>>& macroTokens)
+        : macroInfoMap(macroEvents), macroTokens(macroTokens) {}
     std::unique_ptr<clang::ASTConsumer> CreateASTConsumer(clang::CompilerInstance &CI, llvm::StringRef InFile) override;
     MacroCommentTracker *getTracker() const { return TrackerRaw; }
 
@@ -23,6 +24,7 @@ protected:
 
 private:
     std::unordered_map<clang::FileID, std::map<unsigned, MacroEventInfo>, FileIDHash> &macroInfoMap;
+    std::unordered_map<unsigned, std::vector<TokenInfo>>& macroTokens;
     MacroCommentTracker * TrackerRaw = nullptr; // externally managed in main.cpp
 
 };
