test/snapshots/Pulse_user_defined_predicates1.fst
@@ -8,7 +8,13 @@ open Pulse.Lib.C
 
 
 
-let pts_to_diag (#a:_) (r0 r1:ref a) (v:a) : slprop = (r0 |-> v) ** (r1 |-> v)
+
+let pts_to_diag
+(#a:_)
+(r0 r1:ref a)
+(v:a)
+: slprop
+= (r0 |-> v) ** (r1 |-> v)
 fn double_int
 (r0 : ( ref Int32.t) )
 (r1 : ( ref Int32.t) )
@@ -94,7 +100,10 @@ py = a1})
 {fold point_pred x ({px = a0;
 py = a1}) }
 
-let is_point (p:ref point) (xy : (int & int)) : slprop = exists* v. point_pred p v ** pure (as_int v.px == fst xy) ** pure (as_int v.py == snd xy)
+
+let is_point (p:ref point) (xy : (int & int))
+: slprop
+= exists* v. point_pred p v ** pure (as_int v.px == fst xy) ** pure (as_int v.py == snd xy)
 fn move
 (p : ( ref point) )
 (dx : Int32.t)
@@ -117,7 +126,14 @@ Mkpoint?.py (! (! p)) := (Int32.add (! (! (! p)).py) (! dy));
 point_recover vp; fold (is_point vp (fst v + as_int vdx, snd v + as_int vdy));
 }
 
-ghost fn fold_is_point (p:ref point) (#s:point_spec) requires point_pred p s ensures exists* v. is_point p v ** pure (v == (as_int s.px, as_int s.py)) { fold (is_point p (as_int s.px, as_int s.py)); }
+
+ghost
+fn fold_is_point (p:ref point) (#s:point_spec)
+requires point_pred p s
+ensures exists* v. is_point p v ** pure (v == (as_int s.px, as_int s.py))
+{
+fold (is_point p (as_int s.px, as_int s.py));
+}
 fn move_alt
 (p : ( ref point) )
 (dx : Int32.t)
@@ -166,7 +182,10 @@ unfold is_point;
 (point_free (! p));
 }
 
-let is_point_curry (p:ref point) (x y : int) : slprop = exists* v. point_pred p v ** pure (as_int v.px == x) ** pure (as_int v.py == y)
+
+let is_point_curry (p:ref point) (x y : int)
+: slprop
+= exists* v. point_pred p v ** pure (as_int v.px == x) ** pure (as_int v.py == y)
 fn move_curry
 (p : ( ref point) )
 (dx : Int32.t)
