test/snapshots/Nested_struct_with_arrays.fst
@@ -135,7 +135,23 @@ requires exists* (y: s2). (x |-> y) **
 ensures exists* w. s2_pred x w ** pure (w == {field_s1 = a0})
 {fold s2_pred x ({field_s1 = a0}) }
 
-[@@pulse_unfold] let owns_s2 (x:ref s2) (y:Seq.seq UInt8.t) = exists* s2_spec s1_spec. s2_pred x s2_spec ** s1_pred s2_spec.field_s1 s1_spec ** (s1_spec.bytes |-> y) ** freeable x ** freeable s2_spec.field_s1 ** freeable_array s1_spec.bytes ghost fn intro_owns_s2 (#x:ref s2) (#y:ref s1) (#z:array UInt8.t) (#bytes:Seq.seq UInt8.t) () requires s2_pred x ({field_s1=y}) ** s1_pred y ({bytes=z}) ** (z |-> bytes) ** freeable x ** freeable y ** freeable_array z ensures owns_s2 x bytes { rewrite each z as ({bytes=z}).bytes }
+
+[@@pulse_unfold] let owns_s2 (x:ref s2) (y:Seq.seq UInt8.t) =
+exists* s2_spec s1_spec.
+s2_pred x s2_spec **
+s1_pred s2_spec.field_s1 s1_spec **
+(s1_spec.bytes |-> y) **
+freeable x **
+freeable s2_spec.field_s1 ** freeable_array s1_spec.bytes
+ghost fn intro_owns_s2 (#x:ref s2) (#y:ref s1) (#z:array UInt8.t) (#bytes:Seq.seq UInt8.t) ()
+requires
+s2_pred x ({field_s1=y}) **
+s1_pred y ({bytes=z}) **
+(z |-> bytes) **
+freeable x **
+freeable y **
+freeable_array z
+ensures owns_s2 x bytes { rewrite each z as ({bytes=z}).bytes }
 fn test ()
 {
 let mut size_expr0 : SizeT.t = (uint64_to_sizet (int32_to_uint64 32l));
