test/snapshots/Pulse_tutorial_conditionals.fst
@@ -8,6 +8,7 @@ open Pulse.Lib.C
 
 
 
+
 let max_spec x y = if x < y then y else x
 fn max
 (x : ( ref Int32.t) )
